Current state

Simple_Clause_Learning/Simple_Clause_Learning.thy
@@ -7,7 +7,9 @@ theory Simple_Clause_Learning
     Ordered_Resolution_Prover.Abstract_Substitution
     Ordered_Resolution_Prover.Herbrand_Interpretation
     First_Order_Terms.Unification
-    Functional_Ordered_Resolution_Prover.IsaFoR_Term
+    First_Order_Terms.Subsumption
+    (* Functional_Ordered_Resolution_Prover.IsaFoR_Term *)
+    Abstract_Renaming_Apart
 begin
 
 
@@ -23,8 +25,8 @@ lemma find_map_conv: "find_map f xs = Option.bind (find (\<lambda>x. f x \<noteq
 
 section \<open>Multiset_Extra\<close>
 
-definition msingleton :: "'a \<Rightarrow> 'a multiset" where
-  "msingleton x \<equiv> {#x#}"
+lemma Multiset_Bex_plus_iff: "(\<exists>x \<in># (M1 + M2). P x) \<longleftrightarrow> (\<exists>x \<in># M1. P x) \<or> (\<exists>x \<in># M2. P x)"
+  by auto
 
 
 section \<open>Calculus_Extra\<close>
@@ -35,54 +37,34 @@ lemma (in consequence_relation) entails_one_formula: "N \<Turnstile> U \<Longrig
 
 section \<open>Clausal_Calculus_Extra\<close>
 
-lemma (in substitution) true_cls_thick_substI: "I \<TTurnstile>s N \<cdot>cs \<eta> \<Longrightarrow> D \<in> N \<Longrightarrow> I \<TTurnstile> D \<cdot> \<eta>"
-  by (simp add: substitution_ops.subst_clss_def true_clss_def)
+lemma true_cls_iff_set_mset_eq: "set_mset C = set_mset D \<Longrightarrow> I \<TTurnstile> C \<longleftrightarrow> I \<TTurnstile> D"
+  by (simp add: true_cls_def)
 
-lemma (in substitution) grounding_of_clss_empty[simp]: "grounding_of_clss {} = {}"
+lemma true_clss_if_set_mset_eq: "(\<forall>D \<in> \<D>. \<exists>C \<in> \<C>. set_mset D = set_mset C) \<Longrightarrow> I \<TTurnstile>s \<C> \<Longrightarrow> I \<TTurnstile>s \<D>"
+  using true_cls_iff_set_mset_eq by (metis true_clss_def)
+
+
+section \<open>Abstract_Substitution_Extra\<close>
+
+lemma (in substitution_ops) grounding_of_clss_empty[simp]: "grounding_of_clss {} = {}"
   by (simp add: grounding_of_clss_def)
 
-lemma (in substitution) grounding_of_clss_singleton[simp]:
+lemma (in substitution_ops) grounding_of_clss_singleton[simp]:
   "grounding_of_clss {C} = grounding_of_cls C"
   by (simp add: grounding_of_clss_def)
 
-section \<open>Substitution_Extra\<close>
-
-lemma (in substitution) var_disjoint_ConsD:
-  assumes "var_disjoint (C # Cs)"
-  shows "var_disjoint Cs"
-  unfolding var_disjoint_def
-proof (intro allI impI)
-  fix \<sigma>s :: "'s list"
-  assume "length \<sigma>s = length Cs"
-  then obtain \<tau> where
-    "\<forall>i<Suc (length Cs). \<forall>S. S \<subseteq># (C # Cs) ! i \<longrightarrow> S \<cdot> (id_subst # \<sigma>s) ! i = S \<cdot> \<tau>"
-    using assms[unfolded var_disjoint_def, rule_format, of "id_subst # \<sigma>s"]
-    by auto
-  then show "\<exists>\<tau>. \<forall>i<length Cs. \<forall>S. S \<subseteq># Cs ! i \<longrightarrow> S \<cdot> \<sigma>s ! i = S \<cdot> \<tau>"
-    apply -
-    apply (rule exI[where x = \<tau>])
-    by (metis Suc_less_eq nth_Cons_Suc)
-qed
-
-lemma (in substitution) is_unifiers_insert[simp]:
-  "is_unifiers \<sigma> (insert AA AAA) \<longleftrightarrow> is_unifier \<sigma> AA \<and> is_unifiers \<sigma> AAA"
-  unfolding is_unifiers_def by simp
-
-lemma (in substitution) is_unifier_singleton[simp]: "is_unifier \<sigma> {x}"
-  unfolding is_unifier_def by simp
-
-lemma (in substitution) is_unifiers_image_singleton[simp]: "is_unifiers \<sigma> ((\<lambda>x. {f x}) ` AA)"
-  unfolding is_unifiers_def by simp
+lemma (in substitution_ops) subst_atm_of_eqI:
+  "L \<cdot>l \<sigma> = L' \<cdot>l \<sigma> \<Longrightarrow> atm_of L \<cdot>a \<sigma> = atm_of L' \<cdot>a \<sigma>"
+  by (cases L; cases L') (simp_all add: subst_lit_def)
 
 
 section \<open>First_Order_Terms Extra\<close>
 
 no_notation subst_apply_term (infixl "\<cdot>" 67)
-no_notation subst_apply_literal  (infixl "\<cdot>lit" 60)
-no_notation subst_apply_clause  (infixl "\<cdot>cls" 60)
 no_notation subst_compose (infixl "\<circ>\<^sub>s" 75)
 
-(* notation subst_apply_term (infixl "\<cdot>a" 67) *)
+global_interpretation substitution_ops subst_apply_term Var subst_compose .
+
 notation subst_atm_abbrev (infixl "\<cdot>a" 67)
 notation subst_atm_list (infixl "\<cdot>al" 67)
 notation subst_lit (infixl "\<cdot>l" 67)
@@ -90,70 +72,389 @@ notation subst_cls (infixl "\<cdot>" 67)
 notation subst_clss (infixl "\<cdot>cs" 67)
 notation subst_cls_list (infixl "\<cdot>cl" 67)
 notation subst_cls_lists (infixl "\<cdot>\<cdot>cl" 67)
-notation subst_compose (infixl "\<odot>" 67)
+notation comp_subst_abbrev (infixl "\<odot>" 67)
 
+abbreviation vars_lit :: "('f, 'v) Term.term literal \<Rightarrow> 'v set" where
+  "vars_lit L \<equiv> vars_term (atm_of L)"
 
-section \<open>Abstract Concept of Variable Renaming\<close>
+definition vars_cls :: "('f, 'v) term clause \<Rightarrow> 'v set" where
+  "vars_cls C = Union (set_mset (image_mset vars_lit C))"
 
-locale renaming =
-  fixes renaming :: "'a set \<Rightarrow> 'a \<Rightarrow> 'a"
-  assumes
-    renaming_correct: "finite V \<Longrightarrow> renaming V x \<notin> V" and
-    renaming_inj: "finite V \<Longrightarrow> inj (renaming V)"
+lemma vars_cls_empty[simp]: "vars_cls {#} = {}"
+  unfolding vars_cls_def by simp
 
-definition renaming_nats where
-  "renaming_nats V = (let m = Max V in (\<lambda>x. Suc (x + m)))"
+lemma finite_vars_cls[simp]: "finite (vars_cls C)"
+  unfolding vars_cls_def by simp
 
-subsubsection \<open>Interpretation to Prove That Assumptions Are Consistent\<close>
+lemma vars_cls_plus_iff: "vars_cls (C + D) = vars_cls C \<union> vars_cls D"
+  unfolding vars_cls_def by simp
 
-global_interpretation renaming_nats: renaming renaming_nats
-proof unfold_locales
-  show "\<And>V x. finite V \<Longrightarrow> renaming_nats V x \<notin> V"
-    unfolding renaming_nats_def Let_def by (meson Max.coboundedI Suc_le_lessD not_add_less2)
+lemma is_ground_atm_is_ground_on_var:
+  assumes "is_ground_atm (A \<cdot>a \<sigma>)" and "v \<in> vars_term A"
+  shows "is_ground_atm (\<sigma> v)"
+using assms proof (induction A)
+  case (Var x)
+  then show ?case by auto
 next
-  show "\<And>V. finite V \<Longrightarrow> inj (renaming_nats V)"
-    unfolding renaming_nats_def Let_def by (rule injI) simp
+  case (Fun f ts)
+  then show ?case unfolding is_ground_atm_def
+    by auto
+qed
+
+lemma is_ground_lit_is_ground_on_var:
+  assumes ground_lit: "is_ground_lit (subst_lit L \<sigma>)" and v_in_L: "v \<in> vars_lit L"
+  shows "is_ground_atm (\<sigma> v)"
+proof -
+  let ?A = "atm_of L"
+  from v_in_L have A_p: "v \<in> vars_term ?A"
+    by auto
+  then have "is_ground_atm (?A \<cdot>a \<sigma>)"
+    using ground_lit unfolding is_ground_lit_def by auto
+  then show ?thesis
+    using A_p is_ground_atm_is_ground_on_var by metis
+qed
+
+lemma is_ground_cls_is_ground_on_var:
+  assumes
+    ground_clause: "is_ground_cls (subst_cls C \<sigma>)" and
+    v_in_C: "v \<in> vars_cls C"
+  shows "is_ground_atm (\<sigma> v)"
+proof -
+  from v_in_C obtain L where L_p: "L \<in># C" "v \<in> vars_lit L"
+    unfolding vars_cls_def by auto
+  then have "is_ground_lit (subst_lit L \<sigma>)"
+    using ground_clause unfolding is_ground_cls_def subst_cls_def by auto
+  then show ?thesis
+    using L_p is_ground_lit_is_ground_on_var by metis
+qed
+
+lemma same_on_vars_lit:
+  assumes "\<forall>v \<in> vars_lit L. \<sigma> v = \<tau> v"
+  shows "subst_lit L \<sigma> = subst_lit L \<tau>"
+  using assms
+proof (induction L)
+  case (Pos x)
+  then have "\<forall>v \<in> vars_term x. \<sigma> v = \<tau> v \<Longrightarrow> subst_atm_abbrev x \<sigma> = subst_atm_abbrev x \<tau>"
+    using term_subst_eq by metis+
+  then show ?case
+    unfolding subst_lit_def using Pos by auto
+next
+  case (Neg x)
+  then have "\<forall>v \<in> vars_term x. \<sigma> v = \<tau> v \<Longrightarrow> subst_atm_abbrev x \<sigma> = subst_atm_abbrev x \<tau>"
+    using term_subst_eq by metis+
+  then show ?case
+    unfolding subst_lit_def using Neg by auto
+qed
+
+lemma same_on_vars_clause:
+  assumes "\<forall>v \<in> vars_cls S. \<sigma> v = \<tau> v"
+  shows "subst_cls S \<sigma> = subst_cls S \<tau>"
+  by (smt assms image_eqI image_mset_cong2 mem_simps(9) same_on_vars_lit set_image_mset
+      subst_cls_def vars_cls_def)
+
+global_interpretation substitution "(\<cdot>a)" "Var :: _ \<Rightarrow> ('f, 'v) term" "(\<odot>)"
+proof unfold_locales
+  show "\<And>A. A \<cdot>a Var = A"
+    by auto
+next
+  show "\<And>A \<tau> \<sigma>. A \<cdot>a (\<tau> \<odot> \<sigma>) = A \<cdot>a \<tau> \<cdot>a \<sigma>"
+    by auto
+next
+  show "\<And>\<sigma> \<tau>. (\<And>A. A \<cdot>a \<sigma> = A \<cdot>a \<tau>) \<Longrightarrow> \<sigma> = \<tau>"
+    by (simp add: subst_term_eqI)
+next
+  fix C :: "('f, 'v) term clause" and \<sigma> :: "('f, 'v) subst"
+  assume "is_ground_cls (subst_cls C \<sigma>)"
+  hence ground_atms_\<sigma>: "\<And>v. v \<in> vars_cls C \<Longrightarrow> is_ground_atm (\<sigma> v)"
+    by (meson is_ground_cls_is_ground_on_var)
+
+  define some_ground_trm :: "('f, 'v) term" where "some_ground_trm = (Fun undefined [])"
+  have ground_trm: "is_ground_atm some_ground_trm"
+    unfolding is_ground_atm_def some_ground_trm_def by auto
+  define \<tau> where "\<tau> = (\<lambda>v. if v \<in> vars_cls C then \<sigma> v else some_ground_trm)"
+  then have \<tau>_\<sigma>: "\<forall>v \<in> vars_cls C. \<sigma> v = \<tau> v"
+    unfolding \<tau>_def by auto
+
+  have all_ground_\<tau>: "is_ground_atm (\<tau> v)" for v
+  proof (cases "v \<in> vars_cls C")
+    case True
+    then show ?thesis
+      using ground_atms_\<sigma> \<tau>_\<sigma> by auto
+  next
+    case False
+    then show ?thesis
+      unfolding \<tau>_def using ground_trm by auto
+  qed
+  have "is_ground_subst \<tau>"
+    unfolding is_ground_subst_def
+  proof
+    fix A
+    show "is_ground_atm (A \<cdot>a \<tau>)"
+    proof (induction A)
+      case (Var v)
+      thus ?case using all_ground_\<tau> by auto
+    next
+      case (Fun f As)
+      thus ?case using all_ground_\<tau> by (simp add: is_ground_atm_def)
+    qed
+  qed
+  moreover with \<tau>_\<sigma> have "C \<cdot> \<sigma> = C \<cdot> \<tau>"
+    using same_on_vars_clause by auto
+  ultimately show "\<exists>\<tau>. is_ground_subst \<tau> \<and> C \<cdot> \<tau> = C \<cdot> \<sigma>"
+    by auto
+next
+  show "wfP (strictly_generalizes_atm :: ('f, 'v) term \<Rightarrow> _ \<Rightarrow> _)"
+    unfolding wfP_def
+    by (rule wf_subset[OF wf_subsumes])
+      (auto simp: strictly_generalizes_atm_def generalizes_atm_def term_subsumable.subsumes_def
+        subsumeseq_term.simps)
+qed
+
+definition disjoint_vars where
+  "disjoint_vars C D \<longleftrightarrow> vars_cls C \<inter> vars_cls D = {}"
+
+lemma disjoint_vars_iff_inter_empty: "disjoint_vars C D \<longleftrightarrow> vars_cls C \<inter> vars_cls D = {}"
+  by (rule disjoint_vars_def)
+
+hide_fact disjoint_vars_def
+
+lemma disjoint_vars_sym: "disjoint_vars C D \<longleftrightarrow> disjoint_vars D C"
+  unfolding disjoint_vars_iff_inter_empty by blast
+
+lemma disjoint_vars_plus_iff: "disjoint_vars (C + D) E \<longleftrightarrow> disjoint_vars C E \<and> disjoint_vars D E"
+  unfolding disjoint_vars_iff_inter_empty vars_cls_plus_iff
+  by (simp add: Int_Un_distrib2)
+
+definition disjoint_vars_set where
+  "disjoint_vars_set N \<longleftrightarrow> (\<forall>C \<in> N. \<forall>D \<in> N. C \<noteq> D \<longrightarrow> disjoint_vars C D)"
+
+lemma disjoint_vars_set_substetI[intro]: "disjoint_vars_set N \<Longrightarrow> M \<subseteq> N \<Longrightarrow> disjoint_vars_set M"
+  unfolding disjoint_vars_set_def by auto
+
+lemma inv_renaming_sound:
+  assumes is_var_\<sigma>: "\<And>x. is_Var (\<sigma> x)" and inj_\<sigma>: "inj \<sigma>"
+  shows "\<sigma> \<odot> (Var \<circ> (inv (the_Var \<circ> \<sigma>))) = Var"
+proof -
+  define \<sigma>' where "\<sigma>' = the_Var \<circ> \<sigma>"
+  have \<sigma>_def: "\<sigma> = Var \<circ> \<sigma>'"
+    unfolding \<sigma>'_def using is_var_\<sigma> by auto
+
+  from is_var_\<sigma> inj_\<sigma> have "inj \<sigma>'"
+    unfolding inj_on_def \<sigma>_def comp_def by fast
+  hence "inv \<sigma>' \<circ> \<sigma>' = id"
+    using inv_o_cancel[of \<sigma>'] by simp
+  hence "Var \<circ> (inv \<sigma>' \<circ> \<sigma>') = Var"
+    by simp
+  hence "\<forall>x. (Var \<circ> (inv \<sigma>' \<circ> \<sigma>')) x = Var x"
+    by metis
+  hence "\<forall>x. ((Var \<circ> \<sigma>') \<odot> (Var \<circ> (inv \<sigma>'))) x = Var x"
+    unfolding subst_compose_def by auto
+  thus "\<sigma> \<odot> (Var \<circ> (inv \<sigma>')) = Var"
+    using \<sigma>_def by auto
+qed
+
+lemma ex_inv_subst:
+  assumes is_var_\<sigma>: "\<And>x. is_Var (\<sigma> x)" and inj_\<sigma>: "inj \<sigma>"
+  shows "\<exists>\<tau>. \<sigma> \<odot> \<tau> = Var"
+  using inv_renaming_sound[OF assms] by blast
+
+lemma is_renaming_iff: "is_renaming \<rho> \<longleftrightarrow> (\<forall>x. is_Var (\<rho> x)) \<and> inj \<rho>"
+  (is "?lhs \<longleftrightarrow> ?rhs")
+proof (rule iffI)
+  show "?lhs \<Longrightarrow> ?rhs"
+    unfolding is_renaming_def
+    apply safe
+     apply (metis subst_apply_eq_Var subst_compose term.disc(1))
+    by (metis injI subst_compose_def term.sel(1))
+next
+  show "?rhs \<Longrightarrow> ?lhs"
+    by (auto simp: is_renaming_def intro: ex_inv_subst)
+qed
+
+lemma mgu_subst_range_vars:
+  assumes "Unification.mgu s t = Some \<sigma>"
+  shows "range_vars \<sigma> \<subseteq> vars_term s \<union> vars_term t"
+proof -
+  obtain xs where *: "unify [(s, t)] [] = Some xs" and [simp]: "subst_of xs = \<sigma>"
+    using assms by (simp split: option.splits)
+  from unify_Some_UNIF [OF *] obtain ss
+    where "compose ss = \<sigma>" and "UNIF ss {#(s, t)#} {#}" by auto
+  with UNIF_range_vars_subset [of ss "{#(s, t)#}" "{#}"]
+  show ?thesis using vars_mset_singleton by force
+qed
+
+lemma vars_subst_term: "vars_term (t \<cdot>a \<sigma>) \<subseteq> vars_term t - subst_domain \<sigma> \<union> range_vars \<sigma>"
+proof (induction t)
+  case (Var x)
+  show ?case
+    apply (simp add: range_vars_def subst_domain_def)
+    by (smt (verit, best) SUP_upper Term.term.simps(17) empty_Diff insert_Diff_if le_supI1
+        mem_Collect_eq sup_bot_left sup_ge2)
+next
+  case (Fun f xs)
+  thus ?case by auto
+qed
+
+lemma vars_subst_lit: "vars_lit (L \<cdot>l \<sigma>) \<subseteq> vars_lit L - subst_domain \<sigma> \<union> range_vars \<sigma>"
+  using vars_subst_term[of "atm_of L"] by simp
+
+lemma vars_subst_cls: "vars_cls (C \<cdot> \<sigma>) \<subseteq> vars_cls C - subst_domain \<sigma> \<union> range_vars \<sigma>"
+  unfolding vars_cls_def subst_cls_def
+  apply simp
+  using vars_subst_lit
+  by fastforce
+
+lemma vars_cls_plus[simp]: "vars_cls (C + D) = vars_cls C \<union> vars_cls D"
+  unfolding vars_cls_def by simp
+
+lemma vars_cls_add_mset[simp]: "vars_cls (add_mset L C) = vars_lit L \<union> vars_cls C"
+  by (simp add: vars_cls_def)
+
+lemma vars_cls_subst_mgu_subset:
+  assumes mgu_L_L': "Unification.mgu (atm_of L) (atm_of L') = Some \<eta>"
+  shows "vars_cls ((D + {#L#}) \<cdot> \<eta>) \<subseteq> vars_cls (D + {#L, L'#})"
+proof -
+  have "vars_cls ((D + {#L#}) \<cdot> \<eta>) \<subseteq> vars_cls (D + {#L#}) - subst_domain \<eta> \<union> range_vars \<eta>"
+    by (rule vars_subst_cls[of "(D + {#L#})" \<eta>])
+  also have "... \<subseteq> vars_cls (D + {#L#}) - (vars_lit L \<union> vars_lit L') \<union> vars_lit L \<union> vars_lit L'"
+    using mgu_subst_range_vars[OF mgu_L_L'] mgu_subst_domain[OF mgu_L_L'] by blast
+  also have "... \<subseteq> vars_cls (D + {#L#}) \<union> vars_lit L \<union> vars_lit L'"
+    by fast
+  also have "... \<subseteq> vars_cls D \<union> vars_lit L \<union> vars_lit L'"
+    unfolding vars_cls_plus unfolding vars_cls_def by simp
+  also have "... \<subseteq> vars_cls (D + {#L, L'#})"
+    by auto
+  finally show ?thesis
+    by assumption
+qed
+
+lemma disjoint_vars_set_mgu:
+  assumes
+    disj_N_D_L_L': "disjoint_vars_set N" and
+    D_L_L'_in: "D + {#L, L'#} \<in> N" and
+    mgu_L_L': "Unification.mgu (atm_of L) (atm_of L') = Some \<eta>"
+  shows "disjoint_vars_set (N - {D + {#L, L'#}} \<union> {(D + {#L#}) \<cdot> \<eta>})"
+proof -
+  have vars_D_L_\<eta>_subset: "vars_cls ((D + {#L#}) \<cdot> \<eta>) \<subseteq> vars_cls (D + {#L, L'#})"
+    by (rule vars_cls_subst_mgu_subset[OF mgu_L_L'])
+
+  have disj_D_L_\<eta>: "disjoint_vars ((D + {#L#}) \<cdot> \<eta>) C" if C_in: "C \<in> N - {D + {#L, L'#}}" for C
+  proof -
+    from C_in have "C \<noteq> D + {#L, L'#}" by force
+    hence "disjoint_vars C (D + {#L, L'#})"
+        by (meson D_L_L'_in DiffD1 \<open>C \<in> N - {D + {#L, L'#}}\<close> disj_N_D_L_L' disjoint_vars_set_def)
+    thus ?thesis
+      unfolding disjoint_vars_iff_inter_empty
+      using vars_D_L_\<eta>_subset by blast
+  qed
+
+  show ?thesis
+    unfolding disjoint_vars_set_def
+  proof (intro ballI impI)
+    fix C E
+    assume
+      C_D_in:
+        "C \<in> N - {D + {#L, L'#}} \<union> {(D + {#L#}) \<cdot> \<eta>}"
+        "E \<in> N - {D + {#L, L'#}} \<union> {(D + {#L#}) \<cdot> \<eta>}" and
+      C_neq_E: "C \<noteq> E"
+
+    from C_D_in[unfolded Un_iff] show "disjoint_vars C E"
+    proof (elim disjE)
+      assume "C \<in> N - {D + {#L, L'#}}" and "E \<in> N - {D + {#L, L'#}}"
+      thus "disjoint_vars C E" by (meson C_neq_E DiffE disj_N_D_L_L' disjoint_vars_set_def)
+    next
+      assume "C \<in> {(D + {#L#}) \<cdot> \<eta>}" and "E \<in> {(D + {#L#}) \<cdot> \<eta>}"
+      with \<open>C \<noteq> E\<close> have False by blast
+      thus "disjoint_vars C E" by (rule FalseE)
+    next
+      assume C_in: "C \<in> N - {D + {#L, L'#}}" and E_in: "E \<in> {(D + {#L#}) \<cdot> \<eta>}"
+      thus ?thesis using disj_D_L_\<eta> disjoint_vars_sym by blast
+    next
+      assume C_in: "C \<in> {(D + {#L#}) \<cdot> \<eta>}" and E_in: "E \<in> N - {D + {#L, L'#}}"
+      thus ?thesis using disj_D_L_\<eta> by blast
+    qed
+  qed
+qed
+
+lemma disjoint_vars_set_minus_empty_vars:
+  assumes "vars_cls C = {}"
+  shows "disjoint_vars_set (N - {C}) \<longleftrightarrow> disjoint_vars_set N"
+  using assms unfolding disjoint_vars_set_def disjoint_vars_iff_inter_empty by blast
+
+lemma subst_term_eq_if_mgu:
+  assumes mgu_t_u: "Unification.mgu t u = Some \<mu>"
+  shows "t \<cdot>a \<mu> = u \<cdot>a \<mu>"
+  using mgu_sound[OF mgu_t_u]
+  unfolding Unifiers.is_imgu_def unifiers_def mem_Collect_eq
+  by simp
+
+lemma grounding_of_subst_cls_subset:
+  shows "grounding_of_cls (C \<cdot> \<mu>) \<subseteq> grounding_of_cls C"
+    (is "?lhs \<subseteq> ?rhs")
+proof (rule subsetI)
+  fix D
+  assume "D \<in> ?lhs"
+  then obtain \<gamma> where D_def: "D = C \<cdot> \<mu> \<cdot> \<gamma>" and gr_\<gamma>: "is_ground_subst \<gamma>"
+    unfolding grounding_of_cls_def mem_Collect_eq by auto
+
+  show "D \<in> ?rhs"
+    unfolding grounding_of_cls_def mem_Collect_eq
+    unfolding D_def
+    using is_ground_comp_subst[OF gr_\<gamma>, of \<mu>]
+    by force
 qed
 
 
-subsubsection \<open>Extras Related to First-order Terms\<close>
+subsubsection \<open>Renaming Extra\<close>
 
-context renaming begin
+context renaming_apart begin
 
-lemma Term_is_renaming_Var_renaming: "finite V \<Longrightarrow> Term.is_renaming (Var \<circ> renaming V)"
+lemma inj_Var_renaming: "finite V \<Longrightarrow> inj (Var \<circ> renaming V)"
+  using inj_compose inj_renaming by (metis inj_def term.inject(1))
+
+lemma is_renaming_Var_comp_renaming: "finite V \<Longrightarrow> Term.is_renaming (Var \<circ> renaming V)"
   unfolding Term.is_renaming_def
-  apply simp
-  by (meson comp_inj_on injI inj_on_subset renaming_inj term.inject(1) top_greatest)
+  using inj_Var_renaming by (metis comp_apply inj_on_subset term.disc(1) top_greatest)
 
-lemma is_renaming_Var_renaming: "finite V \<Longrightarrow> is_renaming (Var \<circ> renaming V)"
-  unfolding is_renaming_def
-  using renaming_inj
-  term surj
-  term range
-  oops
-
-lemma vars_term_subst_renaming_disj:
+lemma vars_term_subst_term_Var_comp_renaming_disj:
   assumes fin_V: "finite V"
   shows "vars_term (t \<cdot>a (Var \<circ> renaming V)) \<inter> V = {}"
-  using Term_is_renaming_Var_renaming[OF fin_V] renaming_correct[OF fin_V]
+  using is_renaming_Var_comp_renaming[OF fin_V] renaming_correct[OF fin_V]
   by (induction t) auto
 
 lemma vars_lit_subst_renaming_disj:
   assumes fin_V: "finite V"
   shows "vars_lit (L \<cdot>l (Var \<circ> renaming V)) \<inter> V = {}"
-  using vars_term_subst_renaming_disj[OF fin_V] by auto
+  using vars_term_subst_term_Var_comp_renaming_disj[OF fin_V] by auto
 
 lemma vars_cls_subst_renaming_disj:
   assumes fin_V: "finite V"
-  shows "vars_clause (C \<cdot> (Var \<circ> renaming V)) \<inter> V = {}"
-  unfolding vars_clause_def
+  shows "vars_cls (C \<cdot> (Var \<circ> renaming V)) \<inter> V = {}"
+  unfolding vars_cls_def
   apply simp
   using vars_lit_subst_renaming_disj[OF fin_V]
   by (smt (verit, best) UN_iff UN_simps(10) disjoint_iff multiset.set_map subst_cls_def)
 
+abbreviation renaming_wrt where
+  "renaming_wrt N \<equiv> Var \<circ> renaming (\<Union> (vars_cls ` N))"
+
+definition inv_renaming where
+  "inv_renaming \<rho> \<equiv> Var \<circ> inv (the_Var \<circ> \<rho>)"
+
+lemma inv_renaming_sound: "is_renaming \<rho> \<Longrightarrow> \<rho> \<odot> inv_renaming \<rho> = Var"
+  unfolding is_renaming_iff inv_renaming_def
+  by (auto intro: inv_renaming_sound)
+
+lemma subst_cls_renaming_inv_renaming_idem: "is_renaming \<rho> \<Longrightarrow> C \<cdot> \<rho> \<cdot> inv_renaming \<rho> = C"
+  using inv_renaming_sound
+  by (metis subst_cls_comp_subst subst_cls_id_subst)
+
+lemma is_renaming_renaming_wrt: "finite N \<Longrightarrow> is_renaming (renaming_wrt N)"
+  by (simp add: inj_Var_renaming is_renaming_iff)
+
 definition rename_clause ::
   "('f, 'a) term clause set \<Rightarrow> ('f, 'a) term clause \<Rightarrow> ('f, 'a) term clause" where
-  "rename_clause N C = C \<cdot> (Var \<circ> renaming (\<Union> (vars_clause ` N)))"
+  "rename_clause N C = C \<cdot> renaming_wrt N"
 
 lemma disjoint_vars_set_insert_rename_clause:
   assumes fin_N: "finite N" and disj_N: "disjoint_vars_set N"
@@ -163,57 +464,32 @@ proof (intro ballI impI)
   fix D E
   assume D_in: "D \<in> insert (rename_clause N C) N" and E_in: "E \<in> insert (rename_clause N C) N" and
     D_neq_E: "D \<noteq> E"
-  from fin_N have fin_vars_N: "finite (\<Union> (vars_clause ` N))" by simp
+  from fin_N have fin_vars_N: "finite (\<Union> (vars_cls ` N))" by simp
   show "disjoint_vars D E"
     using D_in E_in D_neq_E
     apply simp
     apply safe
-    unfolding rename_clause_def disjoint_vars_conv
+    unfolding rename_clause_def disjoint_vars_iff_inter_empty
     using vars_cls_subst_renaming_disj[OF fin_vars_N]
-    using disj_N[unfolded disjoint_vars_set_def disjoint_vars_conv, rule_format]
+    using disj_N[unfolded disjoint_vars_set_def disjoint_vars_iff_inter_empty, rule_format]
     by auto
 qed
 
-definition renamings_apart :: "('f, 'a) term clause list \<Rightarrow> ('f, 'a) subst list" where
-  "renamings_apart Cs = replicate (length Cs) (Var \<circ> renaming (\<Union> (vars_clause ` set Cs)))"
+lemma ex_inv_rename_clause: "finite N \<Longrightarrow> \<exists>\<rho>. rename_clause N C \<cdot> \<rho> = C"
+  unfolding rename_clause_def
+  using ex_inv_subst[OF _ inj_Var_renaming]
+  by (metis comp_apply finite_UN finite_vars_cls subst_cls_comp_subst subst_cls_id_subst
+      term.disc(1))
 
-lemma renamings_apart_length: "length (renamings_apart Cs) = length Cs"
-  unfolding renamings_apart_def by simp
-
-lemma renamings_apart_renaming: "\<rho> \<in> set (renamings_apart Cs) \<Longrightarrow> is_renaming \<rho>"
-  unfolding renamings_apart_def
-  apply simp
-  using Term_is_renaming_Var_renaming Term_is_renaming_if_is_renaming
-  find_theorems "is_renaming _ = Term.is_renaming _"
-  oops
-
-lemma renamings_apart_disjoint_vars_set:
-  fixes Cs :: "('f, 'a) term clause list"
-  shows "disjoint_vars_set (set (Cs \<cdot>\<cdot>cl (renamings_apart Cs)))"
-proof (induction Cs)
-  case Nil
-  show ?case
-    by (simp add: renamings_apart_def disjoint_vars_set_def)
-next
-  case (Cons C Cs)
-
-  define \<rho> :: "('f, 'a) subst" where
-    "\<rho> = Var \<circ> renaming (vars_clause C \<union> \<Union> (vars_clause ` set Cs))"
-  have ren_C_Cs_conv: "renamings_apart (C # Cs) = \<rho> # replicate (length Cs) \<rho>"
-    unfolding renamings_apart_def \<rho>_def by simp
-  hence FOO: "(C # Cs) \<cdot>\<cdot>cl renamings_apart (C # Cs) = C \<cdot> \<rho> # Cs \<cdot>\<cdot>cl replicate (length Cs) \<rho>"
-    by (simp add: subst_cls_lists_def)
-
-  have fin_vars_C_Cs: "finite (vars_clause C \<union> \<Union> (vars_clause ` set Cs))"
-    by simp
-
-  show ?case
-    unfolding FOO
-    unfolding disjoint_vars_set_def
-    apply (intro ballI)
-    apply simp
-    apply safe
-    oops
+lemma grounding_of_cls_rename_clause:
+  "finite N \<Longrightarrow> grounding_of_cls (rename_clause N C) = grounding_of_cls C"
+  unfolding grounding_of_cls_def
+  apply (rule Set.equalityI; rule subsetI)
+   apply (metis (no_types) grounding_of_cls_def rename_clause_def subsetD
+      subst_cls_eq_grounding_of_cls_subset_eq)
+  using ex_inv_rename_clause
+  by (smt (verit, ccfv_threshold) Collect_mono_iff grounding_of_cls_def mem_Collect_eq
+      subst_cls_eq_grounding_of_cls_subset_eq)
 
 end
 
@@ -225,12 +501,39 @@ type_synonym ('f, 'v) trail = "(('f, 'v) term literal \<times> ('f, 'v) closure 
 type_synonym ('f, 'v) state =
   "('f, 'v) trail \<times> ('f, 'v) term clause set \<times> nat \<times> ('f, 'v) closure option"
 
+definition clss_of_trail where
+  "clss_of_trail \<Gamma> = (\<Union>Ln \<in> set \<Gamma>. case snd Ln of None \<Rightarrow> {} | Some (D, _) \<Rightarrow> {D})"
+
+lemma clss_of_trail_Nil[simp]: "clss_of_trail [] = {}"
+  by (simp add: clss_of_trail_def)
+
+lemma clss_of_trail_Cons: "clss_of_trail (Ln # \<Gamma>) = clss_of_trail [Ln] \<union> clss_of_trail \<Gamma>"
+  by (simp add: clss_of_trail_def)
+
+lemma finite_clss_of_trail[simp]: "finite (clss_of_trail \<Gamma>)"
+  unfolding clss_of_trail_def
+proof (induction \<Gamma>)
+  case Nil
+  show ?case by simp
+next
+  case (Cons Ln \<Gamma>)
+  then show ?case by (simp add: option.case_eq_if prod.case_eq_if)
+qed
+
 definition trail_propagate ::
   "('f, 'v) trail \<Rightarrow> ('f, 'v) term literal \<Rightarrow> ('f, 'v) closure \<Rightarrow> ('f, 'v) trail" where
   "trail_propagate \<Gamma> L Cl = (L, Some Cl) # \<Gamma>"
 
+lemma clss_of_trail_trail_propagate[simp]:
+  "clss_of_trail (trail_propagate \<Gamma> L (C, \<gamma>)) = clss_of_trail \<Gamma> \<union> {C}"
+  unfolding trail_propagate_def clss_of_trail_def by simp
+
 definition trail_decide :: "('f, 'v) trail \<Rightarrow> ('f, 'v) term literal \<Rightarrow> ('f, 'v) trail" where
   "trail_decide \<Gamma> L = (L, None) # \<Gamma>"
+
+lemma clss_of_trail_trail_decide[simp]:
+  "clss_of_trail (trail_decide \<Gamma> L) = clss_of_trail \<Gamma>"
+  unfolding trail_decide_def clss_of_trail_def by simp
 
 definition is_decision_lit :: "('f, 'v) term literal \<times> ('f, 'v) closure option \<Rightarrow> bool" where
   "is_decision_lit Ln \<longleftrightarrow> snd Ln = None"
@@ -276,6 +579,14 @@ next
     by (cases "is_decision_lit Lc") (simp_all add: suffix_ConsI)
 qed
 
+lemma clss_of_trail_trail_decide_subset:
+  "clss_of_trail (trail_backtrack \<Gamma> n) \<subseteq> clss_of_trail \<Gamma>"
+  unfolding trail_decide_def clss_of_trail_def
+  by (simp add: SUP_subset_mono set_mono_suffix trail_backtrack_suffix)
+
+lemma ball_set_trail_backtrackI: "\<forall>x \<in> set \<Gamma>. P x \<Longrightarrow> \<forall>x \<in> set (trail_backtrack \<Gamma> level). P x"
+  by (meson set_mono_suffix subset_eq trail_backtrack_suffix)
+
 lemma trail_backtrack_hd:
   "trail_backtrack \<Gamma> level = [] \<or> is_decision_lit (hd (trail_backtrack \<Gamma> level))"
   by (induction \<Gamma>) simp_all
@@ -302,17 +613,17 @@ definition trail_false_cls :: "('f, 'v) trail \<Rightarrow> ('f, 'v) term clause
 definition trail_defined_lit :: "('f, 'v) trail \<Rightarrow> ('f, 'v) term literal \<Rightarrow> bool" where
   "trail_defined_lit \<Gamma> L \<longleftrightarrow> (trail_true_lit \<Gamma> L \<or> trail_false_lit \<Gamma> L)"
 
-
-
 lemma ball_trail_backtrackI:
   assumes "\<forall>x \<in> set \<Gamma>. P (fst x)"
   shows "\<forall>x \<in> set (trail_backtrack \<Gamma> i). P (fst x)"
   using assms trail_backtrack_suffix[THEN set_mono_suffix]
   by blast
 
-lemma trail_interp_Cons: "trail_interp (Lc # \<Gamma>) = trail_interp [Lc] \<union> trail_interp \<Gamma>"
-  unfolding trail_interp_def
-  by simp
+lemma trail_interp_Cons: "trail_interp (Ln # \<Gamma>) = trail_interp [Ln] \<union> trail_interp \<Gamma>"
+  unfolding trail_interp_def by simp
+
+lemma trail_interp_Cons': "trail_interp (Ln # \<Gamma>) = (case fst Ln of Pos A \<Rightarrow> {A} | Neg A \<Rightarrow> {}) \<union> trail_interp \<Gamma>"
+  unfolding trail_interp_def by simp
 
 lemma true_lit_thick_unionD: "(I1 \<union> I2) \<TTurnstile>l L \<Longrightarrow> I1 \<TTurnstile>l L \<or> I2 \<TTurnstile>l L"
   by auto
@@ -331,8 +642,6 @@ proof (rule ballI)
     unfolding trail_false_cls_def by simp
   hence "trail_interp ((L, Some Cl) # \<Gamma>) \<TTurnstile>l - M"
     unfolding trail_false_lit_def by simp
-  hence "trail_interp [(L, Some Cl)] \<union> trail_interp \<Gamma> \<TTurnstile>l - M"
-    using trail_interp_Cons by fast
   thus "trail_false_lit \<Gamma> M"
     unfolding trail_false_lit_def
     using M_neq_L
@@ -342,50 +651,33 @@ qed
 
 section \<open>SCL Calculus\<close>
 
-locale scl = renaming renaming_vars
+locale scl = renaming_apart renaming_vars
   for renaming_vars :: "'v set \<Rightarrow> 'v \<Rightarrow> 'v"
-  (* \<comment> \<open>Fiori and Weidenbach (CADE 2019) do not specify whether their mgu is idempotent.\<close>
-  minimal_imgu subst_atm id_subst comp_subst renamings_apart atm_of_atms imgu
-  for
-    subst_atm :: "'a \<Rightarrow> 's \<Rightarrow> 'a" and
-    id_subst :: "'s" and
-    comp_subst :: "'s \<Rightarrow> 's \<Rightarrow> 's" and
-    renamings_apart :: "'a clause list \<Rightarrow> 's list" and
-    atm_of_atms :: "'a list \<Rightarrow> 'a" and
-    imgu :: "'a set set \<Rightarrow> 's option" + *)
-  (* fixes rename_clause :: "('f, 'v) term clause set \<Rightarrow> ('f, 'v) term clause \<Rightarrow> ('f, 'v) term clause" *)
-(*   assumes
-    rename_clause_is_renamed: "rename_clause N C = C' \<Longrightarrow> \<exists>\<sigma>. is_renaming \<sigma> \<and> C' \<cdot> \<sigma> = C" and
-    rename_clause_disjoint_vars_set:
-      "disjoint_vars_set N \<Longrightarrow> disjoint_vars_set (insert (rename_clause N C) N)" and
-    mgu_preserves_disjoint_vars:
-      "finite AAA \<Longrightarrow> \<forall>AA\<in>AAA. finite AA \<Longrightarrow> disjoint_vars_set N \<Longrightarrow> C \<in> N \<Longrightarrow>
-      \<Union> AAA \<subseteq> atms_of C \<Longrightarrow> imgu AAA = Some \<mu> \<Longrightarrow> disjoint_vars_set ((N - {C}) \<union> {C \<cdot> \<mu>})" *)
 begin
 
-(* thm mgu_disjoint_vars_set_subst_clss_ident[no_vars] *)
-
 inductive scl :: "('f, 'v) term clause set \<Rightarrow> ('f, 'v) state => ('f, 'v) state \<Rightarrow> bool" for N where
-  propagate: "C + {#L#} \<in> N \<union> U \<Longrightarrow> is_ground_cls ((C + {#L#}) \<cdot> \<sigma>) \<Longrightarrow>
-    trail_false_cls \<Gamma> (C \<cdot> \<sigma>) \<Longrightarrow> \<not> trail_defined_lit \<Gamma> (L \<cdot>l \<sigma>) \<Longrightarrow>
-    scl N (\<Gamma>, U, k, None) (trail_propagate \<Gamma> (L \<cdot>l \<sigma>) (C + {#L#}, \<sigma>), U, k, None)" |
+  propagate: "C \<in> N \<union> U \<Longrightarrow> C' = rename_clause (N \<union> U \<union> clss_of_trail \<Gamma>) C \<Longrightarrow> C' = C'' + {#L#} \<Longrightarrow>
+    is_ground_cls ((C'' + {#L#}) \<cdot> \<sigma>) \<Longrightarrow> trail_false_cls \<Gamma> (C'' \<cdot> \<sigma>) \<Longrightarrow>
+    \<not> trail_defined_lit \<Gamma> (L \<cdot>l \<sigma>) \<Longrightarrow>
+    scl N (\<Gamma>, U, k, None) (trail_propagate \<Gamma> (L \<cdot>l \<sigma>) (C'' + {#L#}, \<sigma>), U, k, None)" |
 
   decide: "is_ground_lit L \<Longrightarrow> \<not> trail_defined_lit \<Gamma> L \<Longrightarrow>
     scl N (\<Gamma>, U, k, None) (trail_decide \<Gamma> L, U, Suc k, None)" |
 
-  conflict: "D \<in> N \<union> U \<Longrightarrow> D' = rename_clause (N \<union> U) D \<Longrightarrow> is_ground_cls (D' \<cdot> \<sigma>) \<Longrightarrow>
-    trail_false_cls \<Gamma> (D' \<cdot> \<sigma>) \<Longrightarrow>
+  conflict: "D \<in> N \<union> U \<Longrightarrow> D' = rename_clause (N \<union> U \<union> clss_of_trail \<Gamma>) D \<Longrightarrow>
+    is_ground_cls (D' \<cdot> \<sigma>) \<Longrightarrow> trail_false_cls \<Gamma> (D' \<cdot> \<sigma>) \<Longrightarrow>
     scl N (\<Gamma>, U, k, None) (\<Gamma>, U, Suc k, Some (D', \<sigma>))" |
 
   skip: "-(L \<cdot>l \<delta>) \<notin># D \<cdot> \<sigma> \<Longrightarrow>
     scl N (trail_propagate \<Gamma> (L \<cdot>l \<delta>) (C + {#L#}, \<delta>), U, k, Some (D, \<sigma>)) (\<Gamma>, U, k, Some (D, \<sigma>))" |
 
-  factorize: "L \<cdot>l \<sigma> = L' \<cdot>l \<sigma> \<Longrightarrow> Unification.mgu (atm_of L) (atm_of L') = Some \<eta> \<Longrightarrow>
-    scl N (\<Gamma>, U, k, Some (D + {#L,L'#}, \<sigma>)) (\<Gamma>, U, k, Some ((D + {#L#}) \<cdot> \<eta>, \<sigma>))" |
+  factorize: "L \<cdot>l \<sigma> = L' \<cdot>l \<sigma> \<Longrightarrow> Unification.mgu (atm_of L) (atm_of L') = Some \<mu> \<Longrightarrow>
+    scl N (\<Gamma>, U, k, Some (D + {#L,L'#}, \<sigma>)) (\<Gamma>, U, k, Some ((D + {#L#}) \<cdot> \<mu>, \<sigma>))" |
 
   resolve: "\<Gamma> = trail_propagate \<Gamma>' (L \<cdot>l \<delta>) (C + {#L#}, \<delta>) \<Longrightarrow> trail_level_cls \<Gamma> (D \<cdot> \<sigma>) = k \<Longrightarrow>
-    (L \<cdot>l \<delta>) = -(L' \<cdot>l \<sigma>) \<Longrightarrow> Unification.mgu (atm_of L) (atm_of (-L')) = Some \<eta> \<Longrightarrow>
-    scl N (\<Gamma>, U, k, Some (D + {#L'#}, \<sigma>)) (\<Gamma>, U, k, Some ((D + C) \<cdot> \<eta>, \<sigma> \<odot> \<delta>))" |
+    \<rho> = renaming_wrt (N \<union> U \<union> clss_of_trail \<Gamma> \<union> {D + {#L'#}}) \<Longrightarrow>
+    (L \<cdot>l \<delta>) = -(L' \<cdot>l \<sigma>) \<Longrightarrow> Unification.mgu (atm_of L) (atm_of L') = Some \<mu> \<Longrightarrow>
+    scl N (\<Gamma>, U, k, Some (D + {#L'#}, \<sigma>)) (\<Gamma>, U, k, Some ((D + C) \<cdot> \<mu> \<cdot> \<rho>, inv_renaming \<rho> \<odot> \<sigma> \<odot> \<delta>))" |
 
   backtrack: "trail_level_lit \<Gamma> (L \<cdot>l \<sigma>) = k \<Longrightarrow> trail_level_cls \<Gamma> (D \<cdot> \<sigma>) = i \<Longrightarrow>
     scl N (\<Gamma>, U, k, Some (D + {#L#}, \<sigma>)) (trail_backtrack \<Gamma> i, U \<union> {D + {#L#}}, k, None)"
@@ -402,8 +694,8 @@ inductive sound_trail for N U where
   Cons: "\<not> trail_defined_lit \<Gamma> L \<Longrightarrow>
     (case u of
       None \<Rightarrow> True |
-      Some (C, \<sigma>) \<Rightarrow> \<exists>C' L'.
-        C = C' + {#L'#} \<and> L = L' \<cdot>l \<sigma> \<and> trail_false_cls \<Gamma> (C' \<cdot> \<sigma>) \<and> C \<in> N \<union> U) \<Longrightarrow>
+      Some (C, \<sigma>) \<Rightarrow> \<exists>C' L'. C = C' + {#L'#} \<and> L = L' \<cdot>l \<sigma> \<and> trail_false_cls \<Gamma> (C' \<cdot> \<sigma>) \<and>
+        (\<exists>D \<in> N \<union> U. \<exists>\<rho>. is_renaming \<rho> \<and> C = D \<cdot> \<rho>)) \<Longrightarrow>
     sound_trail N U \<Gamma> \<Longrightarrow> sound_trail N U ((L, u) # \<Gamma>)"
 
 lemma sound_trail_supersetI: "sound_trail N U \<Gamma> \<Longrightarrow> N \<subseteq> NN \<Longrightarrow> U \<subseteq> UU \<Longrightarrow> sound_trail NN UU \<Gamma>"
@@ -412,16 +704,44 @@ proof (induction \<Gamma> rule: sound_trail.induct)
   thus ?case by simp
 next
   case (Cons \<Gamma> L u)
-  thus ?case
-    apply simp
-    apply (rule sound_trail.Cons)
-  subgoal
-    by assumption
-  subgoal
-    by (cases u) auto
-  subgoal
-    by simp
-  done
+  show ?case
+  proof (rule sound_trail.Cons)
+    from Cons.hyps show "\<not> trail_defined_lit \<Gamma> L" by simp
+  next
+    from Cons.prems show "sound_trail NN UU \<Gamma>"
+      by (rule Cons.IH)
+  next
+    show
+      "case u of
+        None \<Rightarrow> True
+      | Some (C, \<sigma>) \<Rightarrow>
+        \<exists>C' L'. C = C' + {#L'#} \<and> L = L' \<cdot>l \<sigma> \<and> trail_false_cls \<Gamma> (C' \<cdot> \<sigma>) \<and>
+        (\<exists>D \<in> NN \<union> UU. \<exists>\<rho>. is_renaming \<rho> \<and> C = D \<cdot> \<rho>)"
+    proof (cases u)
+      case None
+      thus ?thesis by simp
+    next
+      case (Some Cl)
+      obtain C \<gamma> where Cl_def: "Cl = (C, \<gamma>)" by force
+      with Cons.hyps Some obtain C' L' where
+        C_def: "C = add_mset L' C'" and L_def: "L = L' \<cdot>l \<gamma>" and
+        tr_false: "trail_false_cls \<Gamma> (C' \<cdot> \<gamma>)" and
+        C_renaing: "\<exists>D \<in> N \<union> U. \<exists>\<rho>. is_renaming \<rho> \<and> C = D \<cdot> \<rho>"
+        by fastforce
+
+      show ?thesis
+        unfolding Some Cl_def option.case prod.case
+      proof (rule exI, rule exI, intro conjI)
+        show "C = C' + {#L'#}" using C_def by simp
+      next
+        show "L = L' \<cdot>l \<gamma>" by (rule L_def)
+      next
+        show "trail_false_cls \<Gamma> (C' \<cdot> \<gamma>)" by (rule tr_false)
+      next
+        show "\<exists>D\<in>NN \<union> UU. \<exists>\<rho>. is_renaming \<rho> \<and> C = D \<cdot> \<rho>" using Cons.prems C_renaing by fast
+      qed
+    qed
+  qed
 qed
 
 lemma sound_trail_backtrackI:
@@ -429,10 +749,24 @@ lemma sound_trail_backtrackI:
   by (induction \<Gamma> rule: sound_trail.induct) (auto intro: sound_trail.intros)
 
 lemma sound_trail_propagate:
-  "sound_trail N U \<Gamma> \<Longrightarrow> \<not> trail_defined_lit \<Gamma> (L \<cdot>l \<sigma>) \<Longrightarrow> trail_false_cls \<Gamma> (C \<cdot> \<sigma>) \<Longrightarrow>
-  C + {#L#} \<in> N \<union> U \<Longrightarrow> sound_trail N U (trail_propagate \<Gamma> (L \<cdot>l \<sigma>) (C + {#L#}, \<sigma>))"
+  assumes
+    sound_\<Gamma>: "sound_trail N U \<Gamma>" and
+    not_tr_def_\<Gamma>_L_\<sigma>: "\<not> trail_defined_lit \<Gamma> (L \<cdot>l \<sigma>)" and
+    tr_false_\<Gamma>_C_\<sigma>: "trail_false_cls \<Gamma> (C \<cdot> \<sigma>)" and
+    ex_renaming: "\<exists>D\<in>N \<union> U. \<exists>\<rho>. is_renaming \<rho> \<and> C + {#L#} = D \<cdot> \<rho>"
+  shows "sound_trail N U (trail_propagate \<Gamma> (L \<cdot>l \<sigma>) (C + {#L#}, \<sigma>))"
   unfolding trail_propagate_def
-  by (rule sound_trail.Cons) auto
+proof (rule sound_trail.Cons; (unfold option.case prod.case)?)
+  show "\<not> trail_defined_lit \<Gamma> (L \<cdot>l \<sigma>)"
+    by (rule not_tr_def_\<Gamma>_L_\<sigma>)
+next
+  show "sound_trail N U \<Gamma>"
+    by (rule sound_\<Gamma>)
+next
+  show "\<exists>C' L'. C + {#L#} = C' + {#L'#} \<and> L \<cdot>l \<sigma> = L' \<cdot>l \<sigma> \<and> trail_false_cls \<Gamma> (C' \<cdot> \<sigma>) \<and>
+    (\<exists>D\<in>N \<union> U. \<exists>\<rho>. is_renaming \<rho> \<and> C + {#L#} = D \<cdot> \<rho>)"
+    using tr_false_\<Gamma>_C_\<sigma> ex_renaming by auto
+qed
 
 lemma sound_trail_decide:
   "sound_trail N U \<Gamma> \<Longrightarrow> \<not> trail_defined_lit \<Gamma> L \<Longrightarrow> sound_trail N U (trail_decide \<Gamma> L)"
@@ -449,7 +783,9 @@ abbreviation entails_\<G> (infix "\<TTurnstile>\<G>e" 50) where
 definition sound_state :: "('f, 'v) Term.term clause set \<Rightarrow> ('f, 'v) state \<Rightarrow> bool" where
   "sound_state N S \<longleftrightarrow> (\<exists>\<Gamma> U k u.
     S = (\<Gamma>, U, k, u) \<and>
-    disjoint_vars_set (N \<union> U \<union> (case u of Some (C, _) \<Rightarrow> {C} | None \<Rightarrow> {})) \<and>
+    finite N \<and> finite U \<and>
+    disjoint_vars_set (N \<union> U \<union> clss_of_trail \<Gamma>) \<and>
+    (case u of None \<Rightarrow> True | Some (C, _) \<Rightarrow> \<forall>D \<in> N \<union> U  \<union> clss_of_trail \<Gamma>. disjoint_vars C D) \<and>
     (\<forall>L \<in> fst ` set \<Gamma>. is_ground_lit L) \<and>
     sound_trail N U \<Gamma> \<and>
     N \<TTurnstile>\<G>e U \<and>
@@ -459,11 +795,8 @@ definition sound_state :: "('f, 'v) Term.term clause set \<Rightarrow> ('f, 'v) 
 abbreviation initial_state :: "('f, 'v) state" where
   "initial_state \<equiv> ([], {}, 0, None)"
 
-lemma sound_initial_state[simp]: "disjoint_vars_set N \<Longrightarrow> sound_state N initial_state"
-  apply (simp add: sound_state_def)
-  apply (intro allI impI)
-  unfolding grounding_of_clss_def
-  by force
+lemma sound_initial_state[simp]: "finite N \<Longrightarrow> disjoint_vars_set N \<Longrightarrow> sound_state N initial_state"
+  by (simp add: sound_state_def)
 
 lemma ball_trail_propagate_is_ground_lit:
   assumes "\<forall>x\<in>set \<Gamma>. is_ground_lit (fst x)" and "is_ground_lit (L \<cdot>l \<sigma>)"
@@ -492,98 +825,116 @@ lemma valid_grounding_of_renaming:
   shows "I \<TTurnstile>s grounding_of_cls (C \<cdot> \<rho>) \<longleftrightarrow> I \<TTurnstile>s grounding_of_cls C"
 proof -
   have "grounding_of_cls (C \<cdot> \<rho>) = grounding_of_cls C" (is "?lhs = ?rhs")
-  proof (rule Set.equalityI)
-    show "?lhs \<subseteq> ?rhs"
-      using subst_cls_eq_grounding_of_cls_subset_eq
-    using assms unfolding is_renaming_def
-  using subset_antisym subst_cls_comp_subst
-      subst_cls_eq_grounding_of_cls_subset_eq subst_cls_id_subst
-      sorry
-  next
-    show "?rhs \<subseteq> ?lhs" sorry
-  qed
+    by (metis (no_types, lifting) assms subset_antisym subst_cls_comp_subst
+        subst_cls_eq_grounding_of_cls_subset_eq subst_cls_id_subst substitution_ops.is_renaming_def)
   thus ?thesis
     by simp
-    unfolding true_clss_def
-    apply (rule ballI)
-    apply (rule \<open>?lhs\<close>[unfolded true_clss_def, rule_format])
-    using assms unfolding is_renaming_def
-  using subset_antisym subst_cls_comp_subst
-      subst_cls_eq_grounding_of_cls_subset_eq subst_cls_id_subst
-  sledgehammer
-  (* by (metis is_renaming_def subset_antisym subst_cls_comp_subst
-      subst_cls_eq_grounding_of_cls_subset_eq subst_cls_id_subst) *)
+qed
 
 theorem scl_sound_state: "scl N S S' \<Longrightarrow> sound_state N S \<Longrightarrow> sound_state N S'"
 proof (induction S S' rule: scl.induct)
-  case (propagate C L U \<sigma> \<Gamma> k)
-  hence "(\<forall>x\<in>set (trail_propagate \<Gamma> (L \<cdot>l \<sigma>) (C + {#L#}, \<sigma>)). is_ground_lit (fst x))"
+  case (propagate C U C' \<Gamma> C'' L \<gamma> k)
+  from propagate.prems have
+    fin: "finite N" "finite U" and
+    disj_N_U_\<Gamma>: "disjoint_vars_set (N \<union> U \<union> clss_of_trail \<Gamma>)" and
+    ball_\<Gamma>_ground: "\<forall>L \<in> set \<Gamma>. is_ground_lit (fst L)" and
+    sound_\<Gamma>: "sound_trail N U \<Gamma>" and
+    N_entails_U: "N \<TTurnstile>\<G>e U"
+    unfolding sound_state_def by auto
+
+  from propagate.hyps have
+    C_in: "C \<in> N \<union> U" and
+    rename_C: "C'' + {#L#} = rename_clause (N \<union> U \<union> clss_of_trail \<Gamma>) C" and
+    gr_C''_L_\<gamma>: "is_ground_cls ((C'' + {#L#}) \<cdot> \<gamma>)"
+    by simp_all
+
+  have "disjoint_vars_set (N \<union> U \<union> clss_of_trail (trail_propagate \<Gamma> (L \<cdot>l \<gamma>) (C'' + {#L#}, \<gamma>)))"
+    using fin disj_N_U_\<Gamma> C_in rename_C by (auto intro: disjoint_vars_set_insert_rename_clause)
+
+  moreover have "\<forall>x\<in>set (trail_propagate \<Gamma> (L \<cdot>l \<gamma>) (C'' + {#L#}, \<gamma>)). is_ground_lit (fst x)"
+  proof (rule ball_trail_propagate_is_ground_lit)
+    show "\<forall>x\<in>set \<Gamma>. is_ground_lit (fst x)"
+      by (rule ball_\<Gamma>_ground)
+  next
+    show "is_ground_lit (L \<cdot>l \<gamma>)"
+      by (rule gr_C''_L_\<gamma>[unfolded is_ground_cls_def, rule_format]) simp
+  qed
+
+  moreover have "sound_trail N U (trail_propagate \<Gamma> (L \<cdot>l \<gamma>) (C'' + {#L#}, \<gamma>))"
+  proof (rule sound_trail_propagate)
+    show "\<exists>D\<in>N \<union> U. \<exists>\<rho>. Simple_Clause_Learning.is_renaming \<rho> \<and> C'' + {#L#} = D \<cdot> \<rho>"
+      unfolding rename_C unfolding rename_clause_def
+      using fin C_in by (metis finite_UnI finite_clss_of_trail is_renaming_renaming_wrt)
+  qed (use propagate.hyps sound_\<Gamma> in simp_all)
+
+  ultimately show ?case
     unfolding sound_state_def
-    by (intro ball_trail_propagate_is_ground_lit) (simp_all add: is_ground_cls_def)
-  with propagate show ?case
-    using sound_trail_propagate
-    by (auto simp: sound_state_def)
+    using fin N_entails_U
+    by simp
 next
   case (decide L \<Gamma> U k)
-  thus ?case
+  from decide.prems have
+    fin: "finite N" "finite U" and
+    disj_N_U_\<Gamma>: "disjoint_vars_set (N \<union> U \<union> clss_of_trail \<Gamma>)" and
+    ball_\<Gamma>_ground: "\<forall>L \<in> set \<Gamma>. is_ground_lit (fst L)" and
+    sound_\<Gamma>: "sound_trail N U \<Gamma>" and
+    N_entails_U: "N \<TTurnstile>\<G>e U"
+    unfolding sound_state_def by auto
+  with decide.hyps show ?case
     unfolding sound_state_def
-    using sound_trail_decide ball_trail_decide_is_ground_lit
-    by fastforce
+    using ball_trail_decide_is_ground_lit[of \<Gamma> L]
+    by (auto intro: sound_trail_decide)
 next
-  case (conflict D U D' \<sigma> \<Gamma> k)
+  case (conflict D U D' \<Gamma> \<sigma> k)
   from conflict.prems have
-    disj_N_U: "disjoint_vars_set (N \<union> U)" and
+    fin_N: "finite N" and
+    fin_U: "finite U" and
+    disj_N_U: "disjoint_vars_set (N \<union> U \<union> clss_of_trail \<Gamma>)" and
     ball_\<Gamma>_ground: "\<forall>L \<in> set \<Gamma>. is_ground_lit (fst L)" and
     sound_\<Gamma>: "sound_trail N U \<Gamma>" and
     N_entails_U: "N \<TTurnstile>\<G>e U"
     unfolding sound_state_def by auto
 
   from conflict.hyps have D_in: "D \<in> N \<union> U" by simp
-  from conflict.hyps have D'_def: "D' = rename_clause (N \<union> U) D" by simp
+  from conflict.hyps have D'_def: "D' = rename_clause (N \<union> U \<union> clss_of_trail \<Gamma>) D" by simp
   from conflict.hyps have tr_false_D': "trail_false_cls \<Gamma> (D' \<cdot> \<sigma>)" by simp
 
-  from disj_N_U and D'_def have disj_N_U_D': "disjoint_vars_set (N \<union> U \<union> {D'})"
-    using rename_clause_disjoint_vars_set by simp
-
-  from D'_def obtain \<rho> where "is_renaming \<rho>" and "D' \<cdot> \<rho> = D"
-      using rename_clause_is_renamed by auto
+  from fin_N fin_U have fin_N_U: "finite (N \<union> U)" by simp
+  with disj_N_U D'_def have disj_N_U_D': "\<forall>C \<in> N \<union> U \<union> clss_of_trail \<Gamma>. disjoint_vars D' C"
+    using disjoint_vars_set_insert_rename_clause
+    by (smt (verit) UN_I Un_iff disjoint_iff disjoint_vars_iff_inter_empty finite_UN finite_UnI
+        finite_clss_of_trail finite_vars_cls rename_clause_def vars_cls_subst_renaming_disj)
 
   have N_entails_D': "N \<TTurnstile>\<G>e {D'}"
   proof (intro allI impI)
-    fix I assume valid_N: "I \<TTurnstile>s grounding_of_clss N"
-    show "I \<TTurnstile>s grounding_of_clss {D'}"
+    fix I
+    assume valid_N: "I \<TTurnstile>s grounding_of_clss N"
+    moreover have "grounding_of_cls D' = grounding_of_cls D"
+      unfolding D'_def
+      using grounding_of_cls_rename_clause fin_N_U
+      by (metis finite_UnI finite_clss_of_trail)
+    ultimately show "I \<TTurnstile>s grounding_of_clss {D'}"
       using D_in
-    proof (rule Set.UnE)
-      assume "D \<in> N"
-      with valid_N have "I \<TTurnstile>s grounding_of_cls D"
-        unfolding grounding_of_clss_def by simp
-      then show ?thesis
-        using \<open>is_renaming \<rho>\<close> \<open>D' \<cdot> \<rho> = D\<close>[symmetric]
-        by (simp add: valid_grounding_of_renaming)
-    next
-      assume "D \<in> U"
-      moreover from N_entails_U valid_N have "I \<TTurnstile>s grounding_of_clss U" by blast
-      ultimately have "I \<TTurnstile>s grounding_of_cls D" by (simp add: grounding_of_clss_def)
-      then show ?thesis
-        using \<open>is_renaming \<rho>\<close> \<open>D' \<cdot> \<rho> = D\<close>[symmetric]
-        by (simp add: valid_grounding_of_renaming)
-    qed
+      by (metis (mono_tags, lifting) N_entails_U UN_I UnE grounding_of_clss_def
+          grounding_of_clss_singleton true_clss_def)
   qed
 
   show ?case
     unfolding sound_state_def
-    using disj_N_U_D' ball_\<Gamma>_ground sound_\<Gamma> N_entails_U tr_false_D' N_entails_D'
+    using fin_N fin_U disj_N_U disj_N_U_D' ball_\<Gamma>_ground sound_\<Gamma> N_entails_U tr_false_D' N_entails_D'
     by simp
 next
   case (skip L \<delta> D \<sigma> \<Gamma> C U k)
   from skip show ?case
     unfolding sound_state_def
-    by (auto simp: trail_propagate_def elim: sound_trail.cases dest!: trail_false_cls_ConsD)
+    by (auto simp: trail_propagate_def clss_of_trail_Cons[of _ \<Gamma>]
+        elim: sound_trail.cases dest!: trail_false_cls_ConsD)
 next
-  case (factorize L \<sigma> L' D \<eta> \<Gamma> U k)
-
+  case (factorize L \<sigma> L' \<mu> \<Gamma> U k D)
   from factorize.prems have
-    disj_N_U_D_L_L': "disjoint_vars_set (N \<union> U \<union> {D + {#L, L'#}})" and
+    fin_N: "finite N" and fin_U: "finite U" and
+    disj_N_U: "disjoint_vars_set (N \<union> U \<union> clss_of_trail \<Gamma>)" and
+    disj_N_U_D_L_L': "\<forall>C \<in> N \<union> U \<union> clss_of_trail \<Gamma>. disjoint_vars (D + {#L, L'#}) C" and
     ball_\<Gamma>_ground:"\<forall>L \<in> set \<Gamma>. is_ground_lit (fst L)" and
     sound_\<Gamma>: "sound_trail N U \<Gamma>" and
     N_entails_U: "N \<TTurnstile>\<G>e U" and
@@ -591,118 +942,343 @@ next
     N_entails_D_L_L': "N \<TTurnstile>\<G>e {D + {#L, L'#}}"
     unfolding sound_state_def by simp_all
 
-  from factorize.hyps have
-    imgu: "imgu (insert {atm_of L, atm_of L'} ((\<lambda>x. {atm_of x}) ` set_mset D)) = Some \<eta>" by simp
+  from factorize.hyps have mgu_L_L': "Unification.mgu (atm_of L) (atm_of L') = Some \<mu>" by simp
+  from factorize.hyps have L_eq_L'_\<sigma>: "L \<cdot>l \<sigma> = L' \<cdot>l \<sigma>" by simp
 
-  from factorize.hyps have unifier_\<sigma>: "is_unifier \<sigma> {atm_of L, atm_of L'}"
-    apply (simp add: is_unifiers_def is_unifier_def subst_lit_def)
-    by (metis atm_of_subst_lit card_1_singleton_iff factorize.hyps(1) image_insert insert_absorb2
-        le_Suc_eq subst_atms_single substitution_ops.subst_atms_def)
-  hence unifiers_\<sigma>: "is_unifiers \<sigma> (insert {atm_of L, atm_of L'} ((\<lambda>x. {atm_of x}) ` set_mset D))" by simp
-  from factorize.hyps have imgu_\<eta>:
-    "is_imgu \<eta> (insert {atm_of L, atm_of L'} ((\<lambda>x. {atm_of x}) ` set_mset D))"
-    by (auto intro: mgu_is_imgu)
-  hence unif_\<mu>: "is_unifier \<eta> {atm_of L, atm_of L'}"
-    using is_unifiers_is_unifier is_mgu_is_unifiers by blast
-  hence "atm_of L \<cdot>a \<eta> = atm_of L' \<cdot>a \<eta>"
-    by (auto intro: is_unifier_subst_atm_eqI[rotated])
-  with factorize.hyps have "L \<cdot>l \<eta> = L' \<cdot>l \<eta>"
-    by (cases L; cases L'; simp add: subst_lit_def)
-  
-  obtain \<gamma> where \<sigma>_def: "\<sigma> = \<eta> \<odot> \<gamma>"
-    using is_mgu_is_most_general[OF is_imgu_is_mgu[OF imgu_\<eta>] unifiers_\<sigma>]
-    by blast
+  hence \<sigma>_unif: "\<sigma> \<in> Unifiers.unifiers {(atm_of L, atm_of L')}"
+    unfolding Unifiers.unifiers_def by (auto intro: subst_atm_of_eqI)
 
-  have "N \<union> U - {add_mset L (add_mset L' D)} = N \<union> U"
-    sorry
+  from mgu_L_L' have L_eq_L'_\<mu>: "L \<cdot>l \<mu> = L' \<cdot>l \<mu>"
+    using subst_term_eq_if_mgu
+    by (metis (mono_tags, lifting) L_eq_L'_\<sigma> atm_of_subst_lit literal.expand subst_lit_is_neg)
 
-  have "(\<Union>x\<in>set_mset D. {atm_of x}) \<subseteq> insert (atm_of L) (insert (atm_of L') (atms_of D))"
-    using atm_of_lit_in_atms_of by fastforce
+  have "disjoint_vars ((D + {#L#}) \<cdot> \<mu>) C" if C_in: "C \<in> N \<union> U \<union> clss_of_trail \<Gamma>" for C
+    using disj_N_U_D_L_L'[rule_format, OF C_in]
+    unfolding _disjoint_vars_iff_inter_empty
+    using vars_cls_subst_mgu_subset[OF mgu_L_L'] 
+    by fast
 
-  then have disj_N_U_D_L: "disjoint_vars_set (N \<union> U \<union> {(D + {#L#}) \<cdot> \<eta>})"
-    using mgu_preserves_disjoint_vars[OF _ _ disj_N_U_D_L_L' _ _ imgu, of "D + {#L, L'#}", simplified]
-    apply (simp add: disjoint_vars_set_insert)
-    using disj_N_U_D_L_L'
-    find_theorems "disjoint_vars_set (insert _ _)"
-    sorry
+  moreover have "trail_false_cls \<Gamma> ((D + {#L#}) \<cdot> \<mu> \<cdot> \<sigma>)"
+    unfolding trail_false_cls_def
+  proof (rule ballI)
 
-  moreover have N_entails_D': "N \<TTurnstile>\<G>e {(D + {#L#}) \<cdot> \<eta>}" sorry
+    fix K
+    assume "K \<in># (D + {#L#}) \<cdot> \<mu> \<cdot> \<sigma>"
+    hence "K \<in># D \<cdot> \<mu> \<cdot> \<sigma> \<or> K = L  \<cdot>l \<mu> \<cdot>l \<sigma>" by force
+    thus "trail_false_lit \<Gamma> K"
+    proof (elim disjE)
+      have is_imgu_\<mu>_full:
+        "Unifiers.is_imgu \<mu> (insert (atm_of L, atm_of L') ((\<lambda>t. (t, t)) ` atm_of ` set_mset D))"
+        sorry
 
-  moreover have "trail_false_cls \<Gamma> ((D + {#L#}) \<cdot> \<eta> \<cdot> \<sigma>)"
-    using imgu_\<eta> tr_false_cls
-    by (simp add: \<sigma>_def trail_false_cls_def \<open>L \<cdot>l \<eta> = L' \<cdot>l \<eta>\<close>)
+      have \<sigma>_unif_full:
+        "\<sigma> \<in> unifiers (insert (atm_of L, atm_of L') ((\<lambda>t. (t, t)) ` atm_of ` set_mset D))"
+        unfolding unifiers_def mem_Collect_eq
+        using L_eq_L'_\<sigma> by (auto intro: subst_atm_of_eqI)
+
+      show "K \<in># D \<cdot> \<mu> \<cdot> \<sigma> \<Longrightarrow> trail_false_lit \<Gamma> K"
+        apply (rule tr_false_cls[unfolded trail_false_cls_def, rule_format])
+        using is_imgu_\<mu>_full \<sigma>_unif_full
+        by (metis (no_types, lifting) Unifiers.is_imgu_def subst_cls_comp_subst subst_cls_union
+            union_iff)
+    next
+      have "L \<cdot>l \<mu> \<cdot>l \<sigma> = L \<cdot>l \<sigma>"
+        using mgu_sound[OF mgu_L_L'] \<sigma>_unif
+        unfolding Unifiers.is_imgu_def
+        by (metis subst_lit_comp_subst)
+      thus "K = L \<cdot>l \<mu> \<cdot>l \<sigma> \<Longrightarrow> trail_false_lit \<Gamma> K"
+        by (auto intro: tr_false_cls[unfolded trail_false_cls_def, rule_format])
+    qed
+  qed
+
+  moreover have "N \<TTurnstile>\<G>e {(D + {#L#}) \<cdot> \<mu>}"
+  proof (rule entails_trans)
+    show "N \<TTurnstile>\<G>e {D + {#L, L'#}}"
+      by (rule N_entails_D_L_L')
+  next
+    have *: "{(D + {#L, L'#}) \<cdot> \<mu>} = {D \<cdot> \<mu> + {#L \<cdot>l \<mu>, L \<cdot>l \<mu>#}}"
+      by (simp add: L_eq_L'_\<mu>)
+
+    have "{D + {#L, L'#}} \<TTurnstile>\<G>e {(D + {#L, L'#}) \<cdot> \<mu>}"
+      using subst_cls_eq_grounding_of_cls_subset_eq true_clss_mono
+      by (metis (mono_tags, lifting) grounding_of_clss_singleton)
+
+    moreover have "{(D + {#L, L'#}) \<cdot> \<mu>} \<TTurnstile>\<G>e {(D + {#L#}) \<cdot> \<mu>}"
+      apply (intro allI impI)
+      by (erule true_clss_if_set_mset_eq[rotated]) (auto simp add: L_eq_L'_\<mu> grounding_of_cls_def)
+
+    ultimately show "{D + {#L, L'#}} \<TTurnstile>\<G>e {(D + {#L#}) \<cdot> \<mu>}"
+      by simp
+  qed
 
   ultimately show ?case
     unfolding sound_state_def
-    using ball_\<Gamma>_ground sound_\<Gamma> N_entails_U
+    using fin_N fin_U disj_N_U ball_\<Gamma>_ground sound_\<Gamma> N_entails_U
     by simp
 next
-  case (resolve \<Gamma> \<Gamma>' L \<delta> C D \<sigma> k L' \<eta> U)
-  from resolve.hyps have imgu_\<eta>: "is_imgu \<eta> {{atm_of L, atm_of L'}}"
-    by (auto intro: mgu_is_imgu)
-
+  case (resolve \<Gamma> \<Gamma>' L \<delta> C D \<sigma> k \<rho> U L' \<mu>)
   from resolve.prems have
-    ball_\<Gamma>_ground_lit: "Ball (fst ` set \<Gamma>) is_ground_lit" and
+    fin: "finite N" "finite U" and
+    disj_N_U: "disjoint_vars_set (N \<union> U \<union> clss_of_trail \<Gamma>)" and
+    disj_N_U_\<Gamma>_D_L_L': "\<forall>C \<in> N \<union> U \<union> clss_of_trail \<Gamma>. disjoint_vars (D + {#L'#}) C" and
+    ball_\<Gamma>_ground:"\<forall>L \<in> set \<Gamma>. is_ground_lit (fst L)" and
     sound_\<Gamma>: "sound_trail N U \<Gamma>" and
-    tr_false_cls_and_entails: "\<And>\<eta>. is_ground_subst \<eta> \<Longrightarrow> N \<cdot>cs \<eta> \<TTurnstile>e U \<cdot>cs \<eta> \<Longrightarrow>
-      trail_false_cls \<Gamma> ((D + {#L'#}) \<cdot> \<sigma>) \<and> N \<cdot>cs \<eta> \<TTurnstile>e {(D + {#L'#}) \<cdot> \<eta>}"
-    unfolding sound_state_def by auto
+    N_entails_U: "N \<TTurnstile>\<G>e U" and
+    tr_false_cls: "trail_false_cls \<Gamma> ((D + {#L'#}) \<cdot> \<sigma>)" and
+    N_entails_D_L': "N \<TTurnstile>\<G>e {D + {#L'#}}"
+    unfolding sound_state_def by simp_all
 
-  from sound_\<Gamma> obtain C' L'' where
-    "\<not> trail_defined_lit \<Gamma>' (L'' \<cdot>l \<delta>)" "sound_trail N U \<Gamma>'" "C + {#L#} = C' + {#L''#}"
-    "- (L' \<cdot>l \<sigma>) = L'' \<cdot>l \<delta>" "trail_false_cls \<Gamma>' (C' \<cdot> \<delta>)" "C + {#L#} \<in> N \<union> U"
-    unfolding resolve.hyps trail_propagate_def
-    apply simp
-    apply (erule sound_trail.cases)
-    by auto 
+  have gr_D_L'_\<sigma>: "is_ground_cls ((D + {#L'#}) \<cdot> \<sigma>)" sorry
+  have tr_undef_\<Gamma>'_L_\<delta>: "\<not> trail_defined_lit \<Gamma>' (L \<cdot>l \<delta>)" sorry
 
-  have "trail_false_cls \<Gamma> ((D + C) \<cdot> \<eta> \<cdot> (\<sigma> \<odot> \<delta>)) \<and> N \<cdot>cs \<eta>' \<TTurnstile>e {(D + C) \<cdot> \<eta> \<cdot> \<eta>'}"
-    (is "?lhs \<and> ?rhs")
-    if ground_\<eta>': "is_ground_subst \<eta>'" and gr_N_entails_U: "N \<cdot>cs \<eta>' \<TTurnstile>e U \<cdot>cs \<eta>'"
-    for \<eta>'
-  proof -
-    have tr_f: "trail_false_cls \<Gamma> ((D + {#L'#}) \<cdot> \<sigma>)" and entails: "N \<cdot>cs \<eta>' \<TTurnstile>e {(D + {#L'#}) \<cdot> \<eta>'}"
-      using tr_false_cls_and_entails[OF ground_\<eta>' gr_N_entails_U] by simp_all
+  from resolve.hyps have L_eq_comp_L': "L \<cdot>l \<delta> = - (L' \<cdot>l \<sigma>)" by simp
+  from resolve.hyps have mgu_L_\<rho>_L': "Unification.mgu (atm_of L) (atm_of L') = Some \<mu>" by simp
+  from resolve.hyps have \<Gamma>_def: "\<Gamma> = trail_propagate \<Gamma>' (L \<cdot>l \<delta>) (C + {#L#}, \<delta>)" by simp
+  from resolve.hyps fin have is_renaming_\<rho>: "is_renaming \<rho>"
+    using is_renaming_renaming_wrt
+    by (metis finite.emptyI finite.insertI finite_UnI finite_clss_of_trail)
 
-    have "\<forall>x\<in>#D \<cdot> \<eta> \<cdot> \<sigma>. trail_false_lit \<Gamma> x"
-      apply (rule ballI)
-      apply (rule tr_f[unfolded trail_false_cls_def, rule_format, simplified])
-      apply (rule disjI2)
-      using imgu_\<eta>
-    proof (elim disjE)
-      sorry
-    have "\<forall>x\<in>#D \<cdot> \<eta> \<cdot> \<sigma> \<cdot> \<delta>. trail_false_lit \<Gamma> x"
-      
-      sorry
-    moreover have "\<forall>x\<in>#C \<cdot> \<eta> \<cdot> \<sigma> \<cdot> \<delta>. trail_false_lit \<Gamma> x"
-      sorry
-    ultimately have "trail_false_cls \<Gamma> ((D + C) \<cdot> \<eta> \<cdot> (\<sigma> \<odot> \<delta>))"
-      by (simp add: trail_false_cls_def ball_Un)
+  have "disjoint_vars ((D + C) \<cdot> \<mu> \<cdot> \<rho>) E" if E_in: "E \<in> N \<union> U \<union> clss_of_trail \<Gamma>" for E
+  proof - 
+    have
+      inter_D_E: "vars_cls D \<inter> vars_cls E = {}" and
+      inter_L'_E: "vars_cls {#L'#} \<inter> vars_cls E = {}"
+        using disj_N_U_\<Gamma>_D_L_L'[rule_format, OF E_in]
+        unfolding disjoint_vars_plus_iff
+        unfolding disjoint_vars_iff_inter_empty
+        by simp_all
 
-    with entails show ?thesis
-      apply simp
-      using \<open>C + {#L#} \<in> N \<union> U\<close>
-      using resolve.hyps 
-      sorry
+    have inter_L_\<rho>_E: "vars_term (atm_of L \<cdot>a \<rho>) \<inter> vars_cls E = {}"
+        by (smt (verit, ccfv_threshold) E_in UN_I UN_Un Un_empty disjoint_iff fin finite.intros
+            finite_UN finite_UnI finite_clss_of_trail finite_vars_cls inf_sup_distrib1
+            vars_lit_subst_renaming_disj resolve.hyps(3) atm_of_subst_lit)
+
+    show ?thesis
+      unfolding subst_cls_union disjoint_vars_plus_iff
+    proof (rule conjI)
+      show "disjoint_vars (D \<cdot> \<mu> \<cdot> \<rho>) E"
+        unfolding disjoint_vars_iff_inter_empty
+        by (smt (verit) E_in UN_I Un_iff disjoint_iff fin finite.intros finite_UN finite_UnI
+            finite_clss_of_trail finite_vars_cls vars_cls_subst_renaming_disj resolve.hyps(3))
+    next
+      show "disjoint_vars (C \<cdot> \<mu> \<cdot> \<rho>) E"
+        unfolding disjoint_vars_iff_inter_empty
+        by (smt (verit) E_in UN_I Un_iff disjoint_iff fin finite.intros finite_UN finite_UnI
+            finite_clss_of_trail finite_vars_cls vars_cls_subst_renaming_disj resolve.hyps(3))
+    qed
   qed
-  with ball_\<Gamma>_ground_lit sound_\<Gamma> show ?case
-    unfolding sound_state_def by simp
+
+  moreover have "trail_false_cls \<Gamma>
+    (D \<cdot> \<mu> \<cdot> \<rho> \<cdot> inv_renaming \<rho> \<cdot> \<sigma> \<cdot> \<delta> + C \<cdot> \<mu> \<cdot> \<rho> \<cdot> inv_renaming \<rho> \<cdot> \<sigma> \<cdot> \<delta>)"
+    unfolding subst_cls_renaming_inv_renaming_idem[OF is_renaming_\<rho>]
+    unfolding trail_false_cls_def
+  proof (rule ballI)
+    have
+      dom_\<sigma>: "subst_domain \<sigma> \<subseteq> vars_cls (D + {#L'#})" and
+      dom_\<delta>: "subst_domain \<delta> \<subseteq> vars_cls (C + {#L#})" sorry
+
+    have vars_D_L'_vars_C_L_disj: "vars_cls (D + {#L'#}) \<inter> vars_cls (C + {#L#}) = {}"
+      apply(rule disj_N_U_\<Gamma>_D_L_L'[unfolded disjoint_vars_iff_inter_empty,
+            rule_format, of "C + {#L#}"])
+      by (simp add: \<Gamma>_def)
+
+    have is_imgu_\<mu>_full:
+      "Unifiers.is_imgu \<mu> (insert (atm_of L, atm_of L')
+        ((\<lambda>t. (t, t)) ` atm_of ` set_mset (C + D)))"
+      sorry
+
+    have \<sigma>_\<delta>_in_unif:"\<sigma> \<odot> \<delta> \<in> unifiers
+          (insert (atm_of L, atm_of L')
+            ((\<lambda>t. (t, t)) ` atm_of ` set_mset (C + D)))" sorry
+
+    have subst_cls_idem_if_disj_vars: "C \<cdot> \<sigma> = C" if "subst_domain \<sigma> \<inter> vars_cls C = {}" for C \<sigma>
+      by (metis (mono_tags, lifting) Int_iff empty_iff mem_Collect_eq same_on_vars_clause
+          subst_cls_id_subst subst_domain_def that)
+
+    fix K
+    assume "K \<in># D \<cdot> \<mu> \<cdot> \<sigma> \<cdot> \<delta> + C \<cdot> \<mu> \<cdot> \<sigma> \<cdot> \<delta>"
+    thus "trail_false_lit \<Gamma> K"
+      unfolding union_iff
+    proof (elim disjE)
+      assume K_in: "K \<in># D \<cdot> \<mu> \<cdot> \<sigma> \<cdot> \<delta>"
+      hence "K \<in># D \<cdot> \<sigma> \<cdot> \<delta>"
+        using is_imgu_\<mu>_full[unfolded Unifiers.is_imgu_def, THEN conjunct2, rule_format,
+            OF \<sigma>_\<delta>_in_unif]
+        by (metis subst_cls_comp_subst)
+      hence "K \<in># D \<cdot> \<sigma>"
+        using gr_D_L'_\<sigma> is_ground_subst_cls by (metis is_ground_cls_union subst_cls_union)
+      then show ?thesis
+        by (auto intro!: tr_false_cls[unfolded trail_false_cls_def, rule_format])
+    next
+      have tr_false_cls_C: "trail_false_cls \<Gamma>' ((C + {#L#}) \<cdot> \<delta>)"
+        using sound_\<Gamma>
+        unfolding sound_trail.simps[of _ _ \<Gamma>]
+        unfolding \<Gamma>_def trail_propagate_def
+        apply simp
+        apply (elim conjE exE)
+        sorry
+
+      assume "K \<in># C \<cdot> \<mu> \<cdot> \<sigma> \<cdot> \<delta>"
+      hence "K \<in># C \<cdot> \<sigma> \<cdot> \<delta>"
+        using is_imgu_\<mu>_full[unfolded Unifiers.is_imgu_def, THEN conjunct2, rule_format,
+            OF \<sigma>_\<delta>_in_unif]
+        by (metis subst_cls_comp_subst)
+      have "K \<in># C \<cdot> \<delta>"
+      proof -
+        have "subst_domain \<sigma> \<inter> vars_cls C = {}"
+          using dom_\<sigma> vars_D_L'_vars_C_L_disj
+          by auto
+        thus ?thesis
+          using \<open>K \<in># C \<cdot> \<sigma> \<cdot> \<delta>\<close> subst_cls_idem_if_disj_vars[of \<sigma> C] by simp
+      qed
+      hence tr_false_\<Gamma>'_K:"trail_false_lit \<Gamma>' K"
+        using tr_false_cls_C[unfolded trail_false_cls_def, rule_format, of K] by simp
+      show ?thesis
+      proof (cases "L \<cdot>l \<delta>")
+        case L_Pos: (Pos t)
+        show ?thesis
+        proof (cases K)
+          case K_Pos: (Pos u)
+          then show ?thesis
+            using L_Pos tr_false_\<Gamma>'_K tr_undef_\<Gamma>'_L_\<delta>
+            unfolding \<Gamma>_def trail_false_lit_def trail_propagate_def trail_defined_lit_def
+              trail_true_lit_def trail_interp_Cons'
+            by simp
+        next
+          case (Neg u)
+          then show ?thesis
+            using L_Pos tr_false_\<Gamma>'_K
+            unfolding \<Gamma>_def trail_false_lit_def trail_propagate_def
+            unfolding trail_interp_Cons' prod.sel
+            by simp
+        qed
+      next
+        case (Neg t)
+        then show ?thesis
+          using tr_false_\<Gamma>'_K
+          unfolding \<Gamma>_def trail_false_lit_def trail_propagate_def
+          unfolding trail_interp_Cons' prod.sel
+          by simp
+      qed
+    qed
+  qed
+
+  moreover have "N \<TTurnstile>\<G>e {(D + C) \<cdot> \<mu> \<cdot> \<rho>}"
+  proof -
+    obtain CC' \<rho>\<^sub>C\<^sub>C where
+      CC'_in: "CC' \<in> N \<union> U" and ren_\<rho>\<^sub>C\<^sub>C: "is_renaming \<rho>\<^sub>C\<^sub>C" and CC'_conv: "C + {#L#} = CC' \<cdot> \<rho>\<^sub>C\<^sub>C"
+      using sound_\<Gamma> unfolding sound_trail.simps[of _ _ \<Gamma>]
+      unfolding \<Gamma>_def trail_propagate_def
+      by auto
+
+    have "N \<TTurnstile>\<G>e {CC'}"
+      using CC'_in
+      by (metis (no_types, opaque_lifting) N_entails_U UnE emptyE grounding_of_clss_mono
+          insert_subset subset_eq true_clss_mono)
+    hence "N \<TTurnstile>\<G>e {CC' \<cdot> \<rho>\<^sub>C\<^sub>C}"
+      using ren_\<rho>\<^sub>C\<^sub>C by (metis valid_grounding_of_renaming grounding_of_clss_singleton)
+    hence "N \<TTurnstile>\<G>e {C + {#L#}}"
+      using CC'_conv by simp
+    hence *: "N \<TTurnstile>\<G>e {(C + {#L#}) \<cdot> \<mu>}"
+      using grounding_of_subst_cls_subset
+      by (metis (no_types, lifting) grounding_of_clss_singleton true_clss_mono)
+
+    have **: "N \<TTurnstile>\<G>e {(D + {#L'#}) \<cdot> \<mu>}"
+      using N_entails_D_L' grounding_of_subst_cls_subset
+      by (metis (no_types, lifting) grounding_of_clss_singleton true_clss_mono)
+
+    have "N \<TTurnstile>\<G>e {(D + C) \<cdot> \<mu>}"
+      unfolding true_clss_def
+    proof (intro allI impI ballI)
+      fix I E
+      assume I_entails: "\<forall>E \<in> grounding_of_clss N. I \<TTurnstile> E" and
+        E_in: "E \<in> grounding_of_clss {(D + C) \<cdot> \<mu>}"
+
+      from E_in have E_in': "E \<in> grounding_of_cls ((D + C) \<cdot> \<mu>)"
+        unfolding grounding_of_clss_def by simp
+      then obtain \<gamma> where E_def: "E = (D + C) \<cdot> \<mu> \<cdot> \<gamma>" and gr_\<gamma>: "is_ground_subst \<gamma>"
+        unfolding grounding_of_cls_def by auto
+
+      have "(D + {#L'#}) \<cdot> \<mu> \<cdot> \<gamma> \<in> grounding_of_clss {(D + {#L'#}) \<cdot> \<mu>}"
+        using gr_\<gamma> unfolding grounding_of_clss_def grounding_of_cls_def by auto
+      hence AA: "\<exists>K \<in># (D + {#L'#}) \<cdot> \<mu> \<cdot> \<gamma>. I \<TTurnstile>l K"
+        using **[rule_format, unfolded true_clss_def, OF I_entails]
+        by (metis true_cls_def)
+
+      have "(C + {#L#}) \<cdot> \<mu> \<cdot> \<gamma> \<in> grounding_of_clss {(C + {#L#}) \<cdot> \<mu>}"
+        using gr_\<gamma> unfolding grounding_of_clss_def grounding_of_cls_def by auto
+      hence BB: "\<exists>K \<in># (C + {#L#}) \<cdot> \<mu> \<cdot> \<gamma>. I \<TTurnstile>l K"
+        using *[rule_format, unfolded true_clss_def, OF I_entails]
+        by (metis true_cls_def)
+
+      show "I \<TTurnstile> E"
+        unfolding E_def true_cls_def
+        using AA[unfolded subst_cls_union Multiset_Bex_plus_iff]
+        using BB[unfolded subst_cls_union Multiset_Bex_plus_iff]
+        unfolding subst_cls_union Multiset_Bex_plus_iff
+      proof (elim disjE)
+        assume "\<exists>K \<in># {#L'#} \<cdot> \<mu> \<cdot> \<gamma>. I \<TTurnstile>l K" and "\<exists>K \<in># {#L#} \<cdot> \<mu> \<cdot> \<gamma>. I \<TTurnstile>l K"
+        hence False
+          using L_eq_comp_L'
+          using subst_term_eq_if_mgu[OF mgu_L_\<rho>_L']
+          by (cases L; cases L'; simp add: uminus_literal_def subst_lit_def)
+        thus "(\<exists>K \<in># D \<cdot> \<mu> \<cdot> \<gamma>. I \<TTurnstile>l K) \<or> (\<exists>K \<in># C \<cdot> \<mu> \<cdot> \<gamma>. I \<TTurnstile>l K)"
+          by simp
+      qed simp_all
+    qed
+    thus ?thesis
+      by (metis (no_types, lifting) grounding_of_clss_singleton grounding_of_subst_cls_subset
+          true_clss_mono)
+  qed
+
+  ultimately show ?case
+    unfolding sound_state_def
+    using fin disj_N_U ball_\<Gamma>_ground sound_\<Gamma> N_entails_U
+    by simp
 next
   case (backtrack \<Gamma> L \<sigma> k D i U)
-  have "\<forall>x\<in>set (trail_backtrack \<Gamma> i). is_ground_lit (fst x)" and
-       N_entails_U: "\<forall>\<eta>. is_ground_subst \<eta> \<longrightarrow> N \<cdot>cs \<eta> \<TTurnstile>e U \<cdot>cs \<eta>" and
-       N_entails_D_plus_L: "\<forall>\<eta>. is_ground_subst \<eta> \<longrightarrow> N \<cdot>cs \<eta> \<TTurnstile>e {D + {#L#}} \<cdot>cs \<eta>"
-    using backtrack.prems
-    by (auto simp: sound_state_def intro!: ball_trail_backtrack_is_ground_litI)
+  from backtrack.prems have
+    fin: "finite N" "finite U" and
+    disj_N_U: "disjoint_vars_set (N \<union> U \<union> clss_of_trail \<Gamma>)" and
+    disj_N_U_\<Gamma>_D_L_L': "\<forall>C \<in> N \<union> U \<union> clss_of_trail \<Gamma>. disjoint_vars (D + {#L#}) C" and
+    ball_\<Gamma>_ground:"\<forall>L \<in> set \<Gamma>. is_ground_lit (fst L)" and
+    sound_\<Gamma>: "sound_trail N U \<Gamma>" and
+    N_entails_U: "N \<TTurnstile>\<G>e U" and
+    tr_false_cls: "trail_false_cls \<Gamma> ((D + {#L#}) \<cdot> \<sigma>)" and
+    N_entails_D_L_L': "N \<TTurnstile>\<G>e {D + {#L#}}"
+    unfolding sound_state_def by simp_all
+
+  have "disjoint_vars_set (N \<union> U \<union> clss_of_trail (trail_backtrack \<Gamma> i) \<union> {D + {#L#}})"
+    unfolding disjoint_vars_set_def
+  proof (intro ballI impI)
+    fix C E
+    assume
+      C_in: "C \<in> N \<union> U \<union> clss_of_trail (trail_backtrack \<Gamma> i) \<union> {D + {#L#}}" and
+      E_in: "E \<in> N \<union> U \<union> clss_of_trail (trail_backtrack \<Gamma> i) \<union> {D + {#L#}}" and
+      C_neq_E: "C \<noteq> E"
+    from C_in have C_in': "C \<in> N \<union> U \<union> clss_of_trail \<Gamma> \<or> C = D + {#L#}"
+      using clss_of_trail_trail_decide_subset by blast
+    from E_in have E_in': "E \<in> N \<union> U \<union> clss_of_trail \<Gamma> \<or> E = D + {#L#}"
+      using clss_of_trail_trail_decide_subset by blast
+    
+    from C_in' E_in' C_neq_E show "disjoint_vars C E"
+      using disj_N_U[unfolded disjoint_vars_set_def, rule_format]
+      using disj_N_U_\<Gamma>_D_L_L' disjoint_vars_sym by blast
+  qed
+
+  moreover have "\<forall>L \<in> set (trail_backtrack \<Gamma> i). is_ground_lit (fst L)"
+    by (rule ball_set_trail_backtrackI[OF ball_\<Gamma>_ground])
+
   moreover have "sound_trail N (insert (add_mset L D) U) (trail_backtrack \<Gamma> i)"
     using backtrack
     by (auto simp: sound_state_def intro: sound_trail_backtrackI sound_trail_supersetI)
-  moreover have "\<And>\<eta>. is_ground_subst \<eta> \<Longrightarrow> N \<cdot>cs \<eta> \<TTurnstile>e (U \<union> {D + {#L#}}) \<cdot>cs \<eta>"
-    using N_entails_U N_entails_D_plus_L
-    by simp
+
+  moreover have "N \<TTurnstile>\<G>e (U \<union> {D + {#L#}})"
+    using N_entails_U N_entails_D_L_L' by (metis UN_Un grounding_of_clss_def true_clss_union)
+
   ultimately show ?case
     unfolding sound_state_def
-    by (simp add: sound_state_def)
+    using fin by simp
 qed
 
 end
